Uniqueness of types (except J).

formalization/uniqueness.v
@@ -3,6 +3,8 @@
 Require Import ett.
 Require Import sanity.
 
+(* Auxiliary admissibility lemmas. *)
+
 Lemma eqctx_sym {G D} : eqctx G D -> eqctx D G.
 Proof.
   intros [|? ? ? ?].  
@@ -30,6 +32,8 @@ Proof.
     + assumption.
 Defined.
 
+(* Auxiliary inversion lemmas. *)
+
 Lemma eqctx_ctxextend G A G' A' :
   eqctx (ctxextend G A) (ctxextend G' A') ->
   ((G = G') * eqtype G A A')%type.
@@ -42,27 +46,42 @@ Proof.
 Defined.
 
 
-(* We need something like this. *)
-Hypothesis substCtxConv :
+(* It looks like we need to strengthen some inference
+   rules, as follows: *)
+
+(* Is this one admissible? *)
+Hypothesis substCtxConv' :
   forall G G' D sbs (E : eqctx G' G),
     issubst sbs G D -> issubst sbs G' D.
 
-(* Hypothesis eqctx_ctx : *)
-(*   forall { G D A }, *)
-(*     eqctx G D -> *)
-(*     eqctx (ctxextend G A) (ctxextend D A). *)
+Hypothesis eqCtxExtend' :
+  forall {G D A B},
+    eqctx G D ->
+    eqtype G A B ->
+    eqctx (ctxextend G A) (ctxextend D B).
 
-Hypothesis eqTyCongWeak :
+Hypothesis eqTyCongWeak' :
   forall { G A A' B B' },
   eqtype G A A' ->
   eqtype G B B' ->
   eqtype (ctxextend G A) (Subst B (sbweak G A)) (Subst B' (sbweak G A')).
 
+Hypothesis eqTyCongZero' :
+  forall {G1 G2 A1 A2 B1 B2 u1 u2},
+    eqctx G1 G2 ->
+    eqtype G1 A1 B1 ->
+    eqterm G1 u1 u2 A1 ->
+    eqtype (ctxextend G1 A1) A2 B2 ->
+    eqtype G1
+           (Subst A2 (sbzero G1 A1 u1))
+           (Subst B2 (sbzero G2 B1 u2)).
+
+(* A hack to be able to admit cases and still have Coq verify
+   that the fixpoints are well-defined. *)
 Hypothesis temporary :
   forall {G A B}, eqtype G A B.
-  
-Hypothesis temporary2 :
-  forall {G D}, eqctx G D.
+
+(* Tactics for dealing with the conversion cases. *)
 
 Ltac doTyConv unique_term' :=
   eapply EqTyTrans ;
@@ -78,7 +97,9 @@ Ltac doCtxConv D' unique_term' :=
   [ eassumption
   | now apply (eqctx_trans _ D') ].
 
-Fixpoint unique_term G u A (H1 : isterm G u A) {struct H1}:
+(* The version of the theorem that allows variation of the context. *)
+
+Fixpoint unique_term_ctx G u A (H1 : isterm G u A) {struct H1}:
   forall B D,
     isterm D u B ->
     eqctx D G ->
@@ -97,13 +118,13 @@ Proof.
     - { 
         apply (@EqTyTrans G _ A B').
         + now apply EqTySym.
-        + eapply (unique_term G u A) ; eassumption.
+        + eapply (unique_term_ctx G u A) ; eassumption.
       }
 
     (* TermCtxConv *)
     - { 
         eapply EqTyCtxConv.
-        - eapply unique_term.
+        - eapply unique_term_ctx.
           + eassumption.
           + eassumption.
           + apply (eqctx_trans _ D).
@@ -119,13 +140,13 @@ Proof.
 
         - eapply CongTySubst.
           + eassumption.
-          + eapply (unique_term _ u).
+          + eapply (unique_term_ctx _ u).
             * exact H1.
             * eassumption.
             * { apply eqctx_sym.
                 apply (unique_subst G _ sbs).
                 - assumption.
-                - eapply substCtxConv.                  
+                - eapply substCtxConv'.
                   + eapply eqctx_sym.
                     eassumption.
                   + assumption. }
@@ -140,7 +161,7 @@ Proof.
             - now rewrite H0.
             - destruct (eqctx_ctxextend _ _ _ _  L) as [E M].
               rewrite E in * |- *.
-              apply eqTyCongWeak.
+              apply eqTyCongWeak'.
               + now apply EqTySym.
               + now apply EqTySym.
           }
@@ -156,9 +177,9 @@ Proof.
               - now rewrite H2.
               - destruct (eqctx_ctxextend _ _ _ _  L) as [E M].
                 rewrite E in * |- *.
-                apply eqTyCongWeak.
+                apply eqTyCongWeak'.
                 + now apply EqTySym.
-                + eapply (unique_term _ (var k)).
+                + eapply (unique_term_ctx _ (var k)).
                   * assumption.
                   * eassumption.
                   * apply eqctx_refl.
@@ -171,8 +192,10 @@ Proof.
           - doTyConv unique_term'.
           - doCtxConv D' unique_term'.
 
-          - now apply temporary.
-
+          - apply EqTyRefl.
+            + apply TyProd.
+              * assumption.
+              * now apply (@sane_isterm (ctxextend G A) B u).
         }
 
       (* TermApp *)
@@ -180,8 +203,12 @@ Proof.
           - doTyConv unique_term'.
           - doCtxConv D' unique_term'.
 
-          - now apply temporary.
-
+          - { apply eqTyCongZero'.
+              - now apply eqctx_sym.
+              - now apply EqTyRefl, (@sane_isterm G A v).
+              - now apply EqRefl.
+              - now apply EqTyRefl.
+            }
         }
 
       (* TermRefl *)
@@ -189,8 +216,10 @@ Proof.
           - doTyConv unique_term'.
           - doCtxConv D' unique_term'.
 
-          - now apply temporary.
-
+          - apply EqTyRefl, TyId.
+            + now apply (@sane_isterm G A u).
+            + assumption.
+            + assumption.
         }
 
       (* TermJ *)
@@ -207,8 +236,10 @@ Proof.
           - doTyConv unique_term'.
           - doCtxConv D' unique_term'.
 
-          - now apply temporary.
-
+          - { apply EqTyRefl.
+              eapply TyCtxConv.
+              + eassumption.
+              + assumption. }
         }
 
       (* TermUnit *)
@@ -216,8 +247,7 @@ Proof.
           - doTyConv unique_term'.
           - doCtxConv D' unique_term'.
 
-          - now apply temporary.
-
+          - now apply EqTyRefl, TyUnit.
         }
 
       (* TermTrue *)
@@ -225,8 +255,7 @@ Proof.
           - doTyConv unique_term'.
           - doCtxConv D' unique_term'.
 
-          - now apply temporary.
-
+          - now apply EqTyRefl, TyBool.
         }
 
       (* TermFalse *)
@@ -234,8 +263,7 @@ Proof.
           - doTyConv unique_term'.
           - doCtxConv D' unique_term'.
 
-          - now apply temporary.
-
+          - now apply EqTyRefl, TyBool.
         }
 
       (* TermCond *)
@@ -243,14 +271,51 @@ Proof.
           - doTyConv unique_term'.
           - doCtxConv D' unique_term'.
 
-          - now apply temporary.
-
+          - { apply eqTyCongZero'.
+              + now apply eqctx_sym.
+              + now apply EqTyRefl, TyBool, (@sane_isterm G Bool u).
+              + now apply EqRefl.
+              + now apply EqTyRefl.
+            }
         }
   }
 
  (* unique_subst *)
- { intros;
-   apply temporary2.
+ { intros D2 H2.
+   destruct H1.
+
+   (* H1: SubstZero *)
+   - { inversion_clear H2.
+       apply eqctx_refl, CtxExtend; now apply (@sane_isterm G A u).
+     }
+
+   (* H1: SubstWeak *)
+   - { inversion_clear H2.
+       now apply eqctx_refl, (@sane_istype D2 A).
+     }
+
+   (* H2: SubstShift *)
+   - { inversion_clear H2.
+       apply eqCtxExtend'.
+       apply (unique_subst G _ sbs).
+       + assumption.
+       + assumption.
+       + now apply EqTyRefl.
+     }       
  }
 
+Defined.
+
+(* The main theorem as it will probably be used. *)
+Corollary unique_term {G A B u} :
+  isterm G u A ->
+  isterm G u B ->
+  eqtype G A B.
+
+Proof.
+  intros H1 H2.
+  eapply unique_term_ctx.
+  - eassumption.
+  - eassumption.
+  - now apply eqctx_refl, (@sane_isterm G A u).
 Defined.
